@prefix cv: <http://data.europa.eu/m8g/> .
@prefix rdfs: <http://www.w3.org/2000/01/rdf-schema#> .
@prefix owl: <http://www.w3.org/2002/07/owl#> .
@prefix rdf: <http://www.w3.org/1999/02/22-rdf-syntax-ns#> .
@prefix xsd: <http://www.w3.org/2001/XMLSchema#> .
@prefix dcat: <http://www.w3.org/ns/dcat#> .
@prefix org: <http://www.w3.org/ns/org#> .
@prefix schema: <http://schema.org/> .
@prefix skos: <http://www.w3.org/2004/02/skos/core#> .
@prefix authsrc: <http://vocab.belgif.be/ns/authsrc#> .

<http://vocab.belgif.be/ns/authsrc#> a owl:Ontology ;
	owl:versionInfo "Draft 2019-04-01" ;
	rdfs:label "AS"@de, "AS"@en, "AS"@fr, "AS"@nl;
	rdfs:comment "Authentischen Quellen"@de, "Authentic Sources"@en, 
		"Sources Authentiques"@fr, "Authentieke bronnen"@nl .

authsrc:Agreement a rdfs:Class, owl:Class ;
	rdfs:isDefinedBy authsrc: ;
	rdfs:label "Accord"@fr, "Agreement"@en, "Overeenkomst"@nl, "Vereinbarung"@de ;
	rdfs:comment "An agreement is a set of statements defining the collaboration between a data provider and one or more data consumers"@en,
		"Een overeenkomst is een reeks verklaringen die de samenwerking tussen een gegevensprovider en een of meer gegevensgebruikers definiëren"@nl,
		"Eine Vereinbarung besteht aus einer Reihe von Anweisungen, die die Zusammenarbeit zwischen einem Datenanbieter und einem oder mehreren Datenkonsumenten definieren"@de,
		"Un accord est un ensemble d'instructions définissant la collaboration entre un fournisseur de données et un ou plusieurs consommateurs de données."@fr .

authsrc:DataElement rdfs:Class, owl:Class ;
	rdfs:isDefinedBy authsrc: ;
	rdfs:label "Data element"@en, "Datenelement"@de, "Gegevenselement"@nl, "Élément de données"@fr .
	rdfs:comment "A data element describes a characteristic (property) or a collection of characteristics (class) of an object. A data element can be authoritative or not. Authoritative data elements have a legal base and have to be reused according to the 'only once' legislation."@en,
		"Een gegevenselement beschrijft een kenmerk (eigenschap) of een verzameling kenmerken (klasse) van een object. Een gegevenselement kan authentiek zijn of niet. Authentieke gegevenselementen hebben een wettelijke basis en moeten opnieuw worden gebruikt volgens de 'only once' wetgeving."@nl,
		"Ein Datenelement beschreibt ein Merkmal (Eigenschaft) oder eine Sammlung von Merkmalen (Klasse) eines Objekts. Ein Datenelement kann authentisch sein oder nicht. Authentische Datenelemente haben eine Rechtsgrundlage und müssen gemäß der 'nur einmal' -Gesetzgebung wiederverwendet werden."@de,
		"Un élément de données décrit une caractéristique (propriété) ou une collection de caractéristiques (classe) d'un objet. Un élément de données peut être authentique ou non. Les éléments de données authentiques ont une base légale et doivent être réutilisés conformément à la législation 'only once'."@fr .


authsrc:DataSource a rdfs:Class, owl:Class ;
	rdfs:isDefinedBy authsrc: ;
	rdfs:label "Data source"@en, "Datenquelle"@de, "Gegevensbron"@nl "Source de données"@fr ;
	rdfs:comment "A Data source is a collection of data elements which describe objects. A data source can be authoritative or not. An authoritative data source contains authoritative data and therefore there is a legal obligation to reuse this data source wherever possible."@en,
		"Een gegevensbron is een verzameling gegevenselementen die objecten beschrijven. Een gegevensbron kan authentiek zijn of niet. Een authentieke gegevensbron bevat authentieke gegevens en daarom is er een wettelijke verplichting om deze gegevensbron waar mogelijk te hergebruiken."@nl,
		"Eine Datenquelle ist eine Sammlung von Datenelementen, die Objekte beschreiben. Eine Datenquelle kann authentisch sein oder nicht. Eine authentische Datenquelle enthält authentische Daten und daher besteht eine gesetzliche Verpflichtung, diese Datenquelle wo immer möglich zu verwenden."@de,
		"Une source de données est une collection d'éléments de données qui décrivent des objets. Une source de données peut être authentique ou non. Une source de données authentique contient des données authentiques et, par conséquent, il existe une obligation légale de réutiliser cette source de données dans la mesure du possible."@fr ;
	rdfs:label "Data source"@en, "Datenquelle"@de, "Gegevensbron"@nl "Source de données"@fr .

authsrc:Initiator a rdfs:Class, owl:Class ;
	rdfs:isDefinedBy authsrc: ;

	rdfs:label  ;
	rdfs:comment .

authsrc:Procedure rdfs:Class, owl:Class ;
	rdfs:isDefinedBy authsrc: ;

	rdfs:label  ;
	rdfs:comment .
	
authsrc:SourceResponsible a rdfs:Class, owl:Class ;
	rdfs:isDefinedBy authsrc: ;

	rdfs:label  ;
	rdfs:comment .
	
gdpr:isDPOInternal a rdf:Property, owl:DataProperty ;
	rdfs:isDefinedBy gdpr: ;
	rdfs:label "DPO interne"@fr, "Internal DPO"@en, "Interne DPO"@nl, "Interner DPO"@de ;
	rdfs:comment "DPO appartient au personnel de l'organisation du contrôleur ou non."@fr, "DPO behoort tot het personeel van de Controller-organisatie of niet."@nl, "DPO belongs to the staff of the Controller organization or not."@en, "DPO gehört dem Personal der Controller-Organisation oder nicht."@de ;
	rdfs:domain gdpr:Controller ;
	rdfs:range xsd:boolean .

authsrc:hasAgreement a rdf:Property, owl:ObjectProperty ;
	rdfs:isDefinedBy authsrc: ;
	rdfs:subPropertyOf dcterms:relation ;
	rdfs:label "Data treatment"@en, "Datenbehandlung"@de, "Gegevensverwerking"@nl, "Traitement des données"@fr ;
	rdfs:domain  ;
	rdfs:range authsrc:Agreement .
